cedar-lean/Cedar/Thm/TPE/ResidualCanError.lean
@@ -1,0 +1,206 @@
+/-
+ Copyright Cedar Contributors
+
+ Licensed under the Apache License, Version 2.0 (the "License");
+ you may not use this file except in compliance with the License.
+ You may obtain a copy of the License at
+
+      https://www.apache.org/licenses/LICENSE-2.0
+
+ Unless required by applicable law or agreed to in writing, software
+ distributed under the License is distributed on an "AS IS" BASIS,
+ WITHOUT WARRANTIES OR CONDITIONS OF ANY KIND, either express or implied.
+ See the License for the specific language governing permissions and
+ limitations under the License.
+-/
+
+import Cedar.TPE
+import Cedar.Thm.WellTyped
+import Cedar.Thm.TPE.Input
+
+namespace Cedar.Spec
+
+inductive Residual.ErrorFree : Residual → Prop where
+  | val : Residual.ErrorFree (.val v ty)
+  | var : Residual.ErrorFree (.var v ty)
+  | mem : Residual.ErrorFree x₁ → Residual.ErrorFree x₂ → Residual.ErrorFree (.binaryApp .mem x₁ x₂ ty)
+  | eq :  Residual.ErrorFree x₁ → Residual.ErrorFree x₂ → Residual.ErrorFree (.binaryApp .eq x₁ x₂ ty)
+  | is : Residual.ErrorFree x₁ → Residual.ErrorFree (.unaryApp (.is _) x₁ ty)
+  | and : Residual.ErrorFree x₁ → Residual.ErrorFree x₂ → Residual.ErrorFree (.and x₁ x₂ ty)
+  -- TODO: Can extend to accept everything that doesn't do arithmetic,
+  -- attribute/tag/hierarchy access, or an extension call.
+
+end Cedar.Spec
+
+namespace Cedar.Thm
+
+open Cedar.Spec
+open Cedar.Validation
+
+theorem error_free_spec (r : Residual) : r.errorFree = true ↔ r.ErrorFree := by
+  cases r
+  any_goals
+    simp only [Residual.errorFree, Bool.false_eq_true, false_iff]
+    intro hc
+    cases hc
+  case val =>
+    simp only [Residual.errorFree, true_iff]
+    constructor
+  case var =>
+    simp only [Residual.errorFree, true_iff]
+    constructor
+  case binaryApp op x₁ x₂ _ =>
+    cases op
+    all_goals
+      simp only [Residual.errorFree, Bool.false_eq_true, Bool.and_eq_true, false_iff ]
+    any_goals
+      intro hc
+      cases hc
+    all_goals
+      have ih₁ := error_free_spec x₁
+      have ih₂ := error_free_spec x₂
+      rw [ih₁, ih₂]
+      constructor
+      · intro ⟨h₁, h₂⟩
+        constructor <;> assumption
+      · intro h
+        cases h
+        rename_i h₁ h₂
+        exact .intro h₁ h₂
+  case unaryApp op x₁ _ =>
+    cases op
+    all_goals
+      simp only [Residual.errorFree, Bool.false_eq_true, false_iff]
+    any_goals
+      intro hc
+      cases hc
+    have ih₁ := error_free_spec x₁
+    rw [ih₁]
+    constructor
+    · intro h₁
+      exact .is h₁
+    · intro h
+      cases h
+      rename_i h
+      exact h
+  case and x₁ x₂ _ =>
+    simp only [Residual.errorFree, Bool.and_eq_true]
+    have ih₁ := error_free_spec x₁
+    have ih₂ := error_free_spec x₂
+    rw [ih₁, ih₂]
+    constructor
+    · intro ⟨h₁, h₂⟩
+      exact .and h₁ h₂
+    · intro h
+      cases h
+      rename_i h₁ h₂
+      exact .intro h₁ h₂
+
+theorem well_typed_residual_eval {r : Residual} :
+  InstanceOfWellFormedEnvironment req es env →
+  Residual.WellTyped env r →
+  (r.evaluate req es) = .error .entityDoesNotExist ∨
+  (r.evaluate req es) = .error .extensionError ∨
+  (r.evaluate req es) = .error .arithBoundsError ∨
+  ∃ v, (r.evaluate req es) = .ok v
+:= by sorry -- by typechecker soundness
+
+theorem error_free_evaluate_ok {r : Residual} :
+  InstanceOfWellFormedEnvironment req es env →
+  Residual.WellTyped env r →
+  r.ErrorFree →
+  (r.evaluate req es).isOk
+:= by
+  intro hwf hwt h₂
+  have heval := well_typed_residual_eval hwf hwt
+  cases h₂
+  · -- val case
+    simp [Residual.evaluate, Except.isOk, Except.toBool]
+  · -- var case
+    rename_i v _
+    cases v <;>
+    simp [Residual.evaluate, Except.isOk, Except.toBool]
+  · -- mem case
+    simp [Residual.evaluate, Except.isOk, Except.toBool]
+    rename_i x₁ x₂ _ he₁ he₂
+    cases hwt
+    rename_i hwt₁ hwt₂ hwt
+    have ih₁ := error_free_evaluate_ok hwf hwt₁ he₁
+    have ih₂ := error_free_evaluate_ok hwf hwt₂ he₂
+    simp [Except.isOk, Except.toBool] at ih₁ ih₂
+    split at ih₁ <;> try contradiction
+    clear ih₁ ; rename_i ih₁
+    split at ih₂ <;> try contradiction
+    clear ih₂ ; rename_i ih₂
+    simp [ih₁, ih₂]
+    simp [apply₂]
+    split
+    all_goals
+      rename_i heval'
+      split at heval'
+    any_goals
+      contradiction
+    any_goals
+      rfl
+    · sorry
+    · sorry
+  · simp [Residual.evaluate, Except.isOk, Except.toBool, apply₂]
+    rename_i x₁ x₂ _ he₁ he₂
+    cases hwt
+    rename_i hwt₁ hwt₂ hwt
+    have ih₁ := error_free_evaluate_ok hwf hwt₁ he₁
+    have ih₂ := error_free_evaluate_ok hwf hwt₂ he₂
+    simp only [Except.isOk, Except.toBool] at ih₁ ih₂
+    split at ih₁ <;> try contradiction
+    clear ih₁ ; rename_i ih₁
+    split at ih₂ <;> try contradiction
+    clear ih₂ ; rename_i ih₂
+    simp [ih₁, ih₂]
+  · -- is case
+    simp [Residual.evaluate, Except.isOk, Except.toBool]
+    rename_i x₁ _ he₁
+    cases hwt with
+    | unaryApp hwt₁ hwt =>
+      have ih₁ := error_free_evaluate_ok hwf hwt₁ he₁
+      simp [Except.isOk, Except.toBool] at ih₁
+      split at ih₁ <;> try contradiction
+      clear ih₁ ; rename_i ih₁
+      simp [ih₁, apply₁]
+      split <;> try rfl
+      rename_i heval'
+      split at heval' <;> try contradiction
+      simp at heval'
+      subst heval'
+      cases hwt
+      simp [Residual.evaluate, ih₁, apply₁]  at heval
+  · simp [Residual.evaluate, Except.isOk, Except.toBool]
+    rename_i x₁ x₂ _ he₁ he₂
+    cases hwt with
+    | and hwt₁ hwt₂ hty₁ hty₂ =>
+      have ih₁ := error_free_evaluate_ok hwf hwt₁ he₁
+      have ih₂ := error_free_evaluate_ok hwf hwt₂ he₂
+      simp [Except.isOk, Except.toBool] at ih₁ ih₂
+      split at ih₁ <;> try contradiction
+      clear ih₁ ; rename_i ih₁
+      split at ih₂ <;> try contradiction
+      clear ih₂ ; rename_i ih₂
+      simp [ih₁, ih₂, Result.as, Coe.coe, Value.asBool]
+      split <;> try rfl
+      rename_i heval'
+      split at heval'
+      · simp at heval'
+        split at heval'
+        · contradiction
+        · have hwts₂ := residual_well_typed_is_sound hwf hwt₂ ih₂
+          rw [hty₂] at hwts₂
+          have ⟨_, hb⟩ := instance_of_anyBool_is_bool hwts₂
+          subst hb
+          simp at heval'
+      · have hwts₁ := residual_well_typed_is_sound hwf hwt₁ ih₁
+        rw [hty₁] at hwts₁
+        have ⟨_, hb⟩ := instance_of_anyBool_is_bool hwts₁
+        subst hb
+        rename_i h_not_bool
+        simp at h_not_bool
+
+end Cedar.Thm
