cedar-lean/Cedar/Thm/TPE/Soundness.lean
@@ -18,6 +18,8 @@ import Cedar.TPE
 import Cedar.Spec
 import Cedar.Validation
 import Cedar.Thm.TPE.Input
+import Cedar.Thm.TPE.ResidualCanError
+import Cedar.Thm.TPE.WellTyped
 import Cedar.Thm.Validation
 import Cedar.Thm.WellTyped
 import Cedar.Thm.Data.Control
@@ -224,6 +226,7 @@ theorem partial_evaluate_is_sound_and
 {pes : PartialEntities}
 {env : TypeEnv}
 (h₂ : InstanceOfWellFormedEnvironment req es env)
+(h₄ : RequestAndEntitiesRefine req es preq pes)
 (hᵢ₁ : Residual.WellTyped env x₁)
 (hᵢ₂ : Residual.WellTyped env x₂)
 (hᵢ₃ : x₁.typeOf = CedarType.bool BoolType.anyBool)
@@ -287,6 +290,61 @@ theorem partial_evaluate_is_sound_and
       simp [h₆] at hᵢ₅
       rcases to_option_left_err hᵢ₅ with ⟨_, hᵢ₅⟩
       simp only [Except.toOption, Result.as, Except.bind_err, hᵢ₅]
+  case _ =>
+    simp [Residual.evaluate]
+    cases h₅ : x₁.evaluate req es
+    · simp [Result.as, Except.toOption]
+      cases h₆ : (TPE.evaluate x₁ preq pes).errorFree <;> simp
+      · split <;> simp
+        rename_i h₇
+        simp [Residual.evaluate] at h₇
+        rw [h₅] at hᵢ₅
+        simp [Except.toOption] at hᵢ₅
+        split at hᵢ₅ <;> try contradiction
+        clear hᵢ₅ ; rename_i hᵢ₅
+        simp [hᵢ₅, Result.as] at h₇
+      · split <;> simp
+        rename_i h₇
+        simp [Residual.evaluate] at h₇
+        subst h₇
+        rw [error_free_spec] at h₆
+        have h₇ : Residual.WellTyped env (TPE.evaluate x₁ preq pes) :=
+          partial_eval_preserves_well_typed h₂ h₄ hᵢ₁
+        have h₈ := error_free_evaluate_ok h₂ h₇ h₆
+        simp [Except.isOk, Except.toBool] at h₈
+        split at h₈ <;> try contradiction
+        clear h₈ ; rename_i h₈
+        rw [h₅, h₈] at hᵢ₅
+        simp [Except.toOption] at hᵢ₅
+    · simp [Result.as, Except.toOption, Coe.coe, Value.asBool]
+      simp [h₅, Except.toOption] at hᵢ₅
+      split at hᵢ₅ <;> try contradiction
+      simp at hᵢ₅
+      subst hᵢ₅
+      rename_i hᵢ₅
+      rename_i v _
+      have ⟨_, hv⟩ : ∃ b, v = .prim (.bool b) := by
+        have h₇ := residual_well_typed_is_sound h₂ hᵢ₁ h₅
+        rw [hᵢ₃] at h₇
+        exact instance_of_anyBool_is_bool h₇
+      subst hv
+      simp only
+      rename_i h₁ _ _ _ _ _
+      simp [h₁, Except.toOption, Residual.evaluate] at hᵢ₆
+      split at hᵢ₆ <;> simp at hᵢ₆
+      subst hᵢ₆
+      rename_i hᵢ₆
+      simp [hᵢ₆]
+      rename_i b _
+      have hb : (if b = false then (Except.ok (Value.prim (Prim.bool b)) : Except Spec.Error _) else Except.ok (Value.prim (Prim.bool false))) = Except.ok (.prim (.bool false)) := by
+        split
+        · rename_i hb
+          simpa using hb
+        · simp
+      simp [hb]
+      rename_i ty _ _ _ _ _
+      cases he : (TPE.evaluate x₁ preq pes).errorFree<;> simp [Residual.evaluate, hᵢ₅, Result.as, Coe.coe, Value.asBool]
+      cases b <;> simp
   case _ =>
     simp [Residual.evaluate]
     generalize h₅ : x₁.evaluate req es = res₁
